Weidenbach_Book/Watched_Literals_Watch_List_Domain_Restart.thy
@@ -76,7 +76,7 @@ lemma remove_all_annot_true_clause_imp_wl_inv_literals_are_\<L>\<^sub>i\<^sub>n:
     L: \<open>literals_are_\<L>\<^sub>i\<^sub>n S\<close>
   shows \<open>literals_are_\<L>\<^sub>i\<^sub>n T\<close>
 proof -
-  obtain S2 T2 S3 where    
+  obtain S2 T2 S3 where
     part_S: \<open>partial_correct_watching S\<close> and
     part_T: \<open>partial_correct_watching T\<close> and
     S_S2: \<open>(S, S2) \<in> state_wl_l None\<close> and
@@ -92,7 +92,7 @@ proof -
     using inv unfolding remove_all_annot_true_clause_imp_wl_inv_def
       remove_all_annot_true_clause_imp_inv_def prod.case
     by blast
-  
+
   obtain T3 where
     T2_T2: \<open>(T2, T3) \<in> twl_st_l None\<close> and
     struct_invs_T3: \<open>twl_struct_invs T3\<close> and
@@ -220,7 +220,7 @@ proof -
   have [refine0]: \<open>replace_annot_in_trail_spec L M \<le> \<Down> Id (replace_annot_in_trail_spec L' M')\<close>
     if \<open>(L, L') \<in> Id\<close> and \<open>(M ,M') \<in> Id\<close> for L L' M M'
     using that by auto
-  have [refine0]: \<open>extract_and_remove N j \<le> \<Down> {((N1, C1, b1), (N1', C1', b1')). 
+  have [refine0]: \<open>extract_and_remove N j \<le> \<Down> {((N1, C1, b1), (N1', C1', b1')).
          N1' = fmdrop j N \<and> C1' = N\<propto>j \<and>
          b1 = irred N j \<and> N1 = N1' \<and> C1 = C1' \<and> b1 = b1'} (extract_and_remove N' j')\<close>
        (is \<open>_ \<le> \<Down> ?extract_and_remove _\<close>)
@@ -230,7 +230,7 @@ proof -
     by (auto simp: extract_and_remove_def intro_spec_refine_iff
         intro!: ASSERT_refine_left RES_refine)
   have x1_Lall: \<open>x1 \<in># \<L>\<^sub>a\<^sub>l\<^sub>l\<close>
-    if 
+    if
       pre: \<open>remove_one_annot_true_clause_one_imp_wl_pre L'
       (M', N0', D', NE0', UE', Q', W')\<close> and
       x1: \<open>rev M' ! L' = Propagated x1 x2\<close> and
@@ -300,7 +300,7 @@ proof -
          C1' = N0 \<propto> x2a \<and>
          b1 = irred N0 x2a \<and>
          N1 = N1' \<and> C1 = C1' \<and> b1 = b1'}\<close> and
-      st: 
+      st:
         \<open>x2b = (x1c, x2c)\<close>
         \<open>x'a = (x1b, x2b)\<close>
         \<open>x2d = (x1e, x2e)\<close>
@@ -311,31 +311,31 @@ proof -
       x2c x1d x2d x1e x2e L M N0 D NE0 UE Q W L' M' N0' D' NE0' UE' Q' W'
   proof -
     have st':
-      \<open>x2b = (N0' \<propto> x2a, irred N0' x2a)\<close> 
-      \<open>x'a = (fmdrop x2a N0', N0' \<propto> x2a, irred N0' x2a)\<close> 
-      \<open>x2d = the (fmlookup N0' x2a)\<close> 
-      \<open>xa = (fmdrop x2a N0', the (fmlookup N0' x2a))\<close> 
-      \<open>x' = (x1, x2)\<close> 
-      \<open>Ma = Maa\<close> 
-      \<open>x = (x1, x2)\<close> 
-      \<open>x1b = fmdrop x2a N0'\<close> 
-      \<open>L = L'\<close> 
-      \<open>x1c = N0' \<propto> x2a\<close> 
-      \<open>M = M'\<close> 
-      \<open>N0 = N0'\<close> 
-      \<open>x1d = fmdrop x2a N0'\<close> 
-      \<open>D = D'\<close> 
-      \<open>x1e = N0' \<propto> x2a\<close> 
-      \<open>NE0 = NE0'\<close> 
-      \<open>UE = UE'\<close> 
-      \<open>Q = Q'\<close> 
-      \<open>W = W'\<close> 
+      \<open>x2b = (N0' \<propto> x2a, irred N0' x2a)\<close>
+      \<open>x'a = (fmdrop x2a N0', N0' \<propto> x2a, irred N0' x2a)\<close>
+      \<open>x2d = the (fmlookup N0' x2a)\<close>
+      \<open>xa = (fmdrop x2a N0', the (fmlookup N0' x2a))\<close>
+      \<open>x' = (x1, x2)\<close>
+      \<open>Ma = Maa\<close>
+      \<open>x = (x1, x2)\<close>
+      \<open>x1b = fmdrop x2a N0'\<close>
+      \<open>L = L'\<close>
+      \<open>x1c = N0' \<propto> x2a\<close>
+      \<open>M = M'\<close>
+      \<open>N0 = N0'\<close>
+      \<open>x1d = fmdrop x2a N0'\<close>
+      \<open>D = D'\<close>
+      \<open>x1e = N0' \<propto> x2a\<close>
+      \<open>NE0 = NE0'\<close>
+      \<open>UE = UE'\<close>
+      \<open>Q = Q'\<close>
+      \<open>W = W'\<close>
       \<open>x2e = irred N0' x2a\<close>
       \<open>x2c = x2e\<close>
       using st eq eq'
       by (cases \<open>the (fmlookup N0' x2a)\<close>; auto)+
     have [simp]: \<open>x1a = x1\<close>
-      using \<open>x = (x1a, x2a)\<close> unfolding \<open>x = (x1, x2)\<close> 
+      using \<open>x = (x1a, x2a)\<close> unfolding \<open>x = (x1, x2)\<close>
       by auto
     obtain x xa where
       L: \<open>literals_are_\<L>\<^sub>i\<^sub>n (M, N0, D, NE0, UE, Q, W)\<close> and
@@ -364,7 +364,7 @@ proof -
     have \<open>atm_of (lit_of (rev M ! L)) \<in># \<A>\<^sub>i\<^sub>n\<close>
       using le' by (auto simp: rev_nth lits_of_def in_\<L>\<^sub>a\<^sub>l\<^sub>l_atm_of_\<A>\<^sub>i\<^sub>n)
     then have \<open>x1a \<in># \<L>\<^sub>a\<^sub>l\<^sub>l\<close>
-      using lit x unfolding st' by (auto simp: in_\<L>\<^sub>a\<^sub>l\<^sub>l_atm_of_\<A>\<^sub>i\<^sub>n st state_wl_l_def st 
+      using lit x unfolding st' by (auto simp: in_\<L>\<^sub>a\<^sub>l\<^sub>l_atm_of_\<A>\<^sub>i\<^sub>n st state_wl_l_def st
           split: if_splits)
     then show ?thesis
       using x \<open>x2a \<in># dom_m N0\<close> L unfolding st by (auto simp: st' ran_m_fmdrop
@@ -432,34 +432,47 @@ proof -
 qed
 
 definition mark_to_delete_clauses_wl_D_pre where
-  \<open>mark_to_delete_clauses_wl_D_pre S \<longleftrightarrow> literals_are_\<L>\<^sub>i\<^sub>n S\<close>
+  \<open>mark_to_delete_clauses_wl_D_pre S \<longleftrightarrow> mark_to_delete_clauses_wl_pre S \<and> literals_are_\<L>\<^sub>i\<^sub>n S\<close>
 
 definition mark_to_delete_clauses_wl_D_inv where
-  \<open>mark_to_delete_clauses_wl_D_inv = (\<lambda>(M, N0, D, NE, UE, Q, W) (b, i, N).
-       mark_to_delete_clauses_wl_inv (M, N0, D, NE, UE, Q, W) (b, i, N) \<and>
+  \<open>mark_to_delete_clauses_wl_D_inv = (\<lambda>(M, N0, D, NE, UE, Q, W) xs0 (b, i, N, xs).
+       mark_to_delete_clauses_wl_inv (M, N0, D, NE, UE, Q, W) xs0 (b, i, N, xs) \<and>
         literals_are_\<L>\<^sub>i\<^sub>n (M, N, D, NE, UE, Q, W))\<close>
 
 definition mark_to_delete_clauses_wl_D :: \<open>nat twl_st_wl \<Rightarrow> nat twl_st_wl nres\<close> where
 \<open>mark_to_delete_clauses_wl_D  = (\<lambda>(M, N, D, NE, UE, Q, W). do {
     ASSERT(mark_to_delete_clauses_wl_D_pre (M, N, D, NE, UE, Q, W));
-    xs \<leftarrow> collect_valid_indices_wl (M, N, D, NE, UE, Q, W);
-    (_, _, N) \<leftarrow> WHILE\<^sub>T\<^bsup>mark_to_delete_clauses_wl_D_inv (M, N, D, NE, UE, Q, W)\<^esup>
-      (\<lambda>(brk, i, N). \<not>brk \<and> i < length xs)
-      (\<lambda>(brk, i, N). do {
-        ASSERT(N\<propto>(xs!i)!0 \<in># \<L>\<^sub>a\<^sub>l\<^sub>l);
-        can_del \<leftarrow> SPEC(\<lambda>b. b \<longrightarrow> (Propagated (N\<propto>(xs!i)!0) (xs!i) \<notin> set M) \<and> \<not>irred N (xs!i));
-        brk \<leftarrow> SPEC(\<lambda>_. True);
-        ASSERT(i < length xs);
-        if can_del
-        then
-          RETURN (brk, i+1, fmdrop (xs!i) N)
-        else
-          RETURN (brk, i+1, N)
+    xs0 \<leftarrow> collect_valid_indices_wl (M, N, D, NE, UE, Q, W);
+    (_, _, N, _) \<leftarrow> WHILE\<^sub>T\<^bsup>mark_to_delete_clauses_wl_D_inv (M, N, D, NE, UE, Q, W) xs0\<^esup>
+      (\<lambda>(brk, i, N, xs). \<not>brk \<and> i < length xs)
+      (\<lambda>(brk, i, N, xs). do {
+        if(xs!i \<notin># dom_m N) then RETURN (brk, i, N, delete_index_and_swap xs i)
+        else do {
+          ASSERT(0 < length (N\<propto>(xs!i)));
+          ASSERT(N\<propto>(xs!i)!0 \<in># \<L>\<^sub>a\<^sub>l\<^sub>l);
+          can_del \<leftarrow> SPEC(\<lambda>b. b \<longrightarrow> (Propagated (N\<propto>(xs!i)!0) (xs!i) \<notin> set M) \<and> \<not>irred N (xs!i));
+          brk \<leftarrow> SPEC(\<lambda>_. True);
+          ASSERT(i < length xs);
+          if can_del
+          then
+            RETURN (brk, i+1, fmdrop (xs!i) N, xs)
+          else
+            RETURN (brk, i+1, N, xs)
+        }
       })
-      (False, 0, N);
+      (False, 0, N, xs0);
     RETURN (M, N, D, NE, UE, Q, W)
   })\<close>
- 
+
+lemma (in -) Union_bool_expand: \<open>(\<Union>can_del\<in>{b::bool. P b}. f can_del) =
+   ((if P True then f True else {}) \<union> (if P False then f False else {})) \<close>
+  apply auto
+  apply (case_tac can_del; solves \<open>auto\<close>)
+  apply (case_tac can_del; solves \<open>auto\<close>)
+  apply (case_tac can_del; solves \<open>auto\<close>)
+  apply (case_tac x; solves \<open>auto\<close>)
+  done
+
 lemma mark_to_delete_clauses_wl_D_mark_to_delete_clauses_wl:
   \<open>(mark_to_delete_clauses_wl_D, mark_to_delete_clauses_wl) \<in>
    {(S, T). (S, T) \<in> Id \<and> literals_are_\<L>\<^sub>i\<^sub>n S} \<rightarrow>\<^sub>f
@@ -470,53 +483,459 @@ proof -
     using that by auto
   have [iff]: \<open>(\<forall>(x::bool) xa. P x xa) \<longleftrightarrow> (\<forall>xa.( P True xa \<and> P False xa))\<close> for P
     by metis
+
+  have R_notin: \<open>((brk, i, N, delete_index_and_swap xs i), brk', i', N',
+       delete_index_and_swap xs' i')
+      \<in> {((brk, i, N, xs), brk', i', N', xs').
+          brk = brk' \<and>
+          i = i' \<and>
+          N = N' \<and>
+          xs = xs' \<and> mark_to_delete_clauses_wl_D_inv S xs0 (brk, i, N, xs)}\<close>
+    if
+      T: \<open>T = (SM, SN, SD, SNE, SUE, SQ, SW)\<close> and
+      S: \<open>S = (SM, SN, SD, SNE, SUE, SQ, SW)\<close> and
+      \<open>literals_are_\<L>\<^sub>i\<^sub>n (SM, SN, SD, SNE, SUE, SQ, SW)\<close> and
+      \<open>mark_to_delete_clauses_wl_D_pre (SM, SN, SD, SNE, SUE, SQ, SW)\<close> and
+      xs: \<open>(xs0, xs0') \<in> {(N, N'). N = N' \<and> distinct N}\<close> and
+      \<open>xs0 \<in> {N. distinct N}\<close> and
+      \<open>xs0' \<in> {N. distinct N}\<close> and
+      ss': \<open>(s, s') \<in> {((brk, i, N, xs), brk', i', N', xs'). brk = brk' \<and> i = i' \<and> N = N' \<and>
+         xs = xs' \<and> mark_to_delete_clauses_wl_D_inv S xs0 (brk, i, N, xs)}\<close> and
+      \<open>case s of (brk, i, N, xs) \<Rightarrow> \<not> brk \<and> i < length xs\<close> and
+      \<open>case s' of (brk, i, N, xs) \<Rightarrow> \<not> brk \<and> i < length xs\<close> and
+      inv: \<open>mark_to_delete_clauses_wl_D_inv (SM, SN, SD, SNE, SUE, SQ, SW) xs0 s\<close> and
+      \<open>mark_to_delete_clauses_wl_inv (SM, SN, SD, SNE, SUE, SQ, SW) xs0' s'\<close> and
+      post_inv: \<open>(case s' of (brk, i, N, xs) \<Rightarrow>
+        if xs ! i \<notin># dom_m N
+        then RETURN (brk, i, N, delete_index_and_swap xs i)
+        else ASSERT (0 < length (N \<propto> (xs ! i))) \<bind>
+            (\<lambda>_. SPEC (\<lambda>b. b \<longrightarrow> Propagated (N \<propto> (xs ! i) ! 0) (xs ! i) \<notin> set SM \<and>
+                   \<not> irred N (xs ! i)) \<bind>
+             (\<lambda>can_del. SPEC (\<lambda>_. True) \<bind>
+                 (\<lambda>brk. ASSERT (i < length xs) \<bind>
+                        (\<lambda>_. if can_del
+                             then RETURN (brk, i + 1, fmdrop (xs ! i) N, xs)
+                             else RETURN (brk, i + 1, N, xs))))))
+     \<le> SPEC (mark_to_delete_clauses_wl_inv (SM, SN, SD, SNE, SUE, SQ, SW)
+               xs0')\<close> and
+      st:
+        \<open>si' = (N', xs')\<close>
+        \<open>sbrk' = (i', si')\<close>
+        \<open>s' = (brk', sbrk')\<close>
+        \<open>si = (N, xs)\<close>
+        \<open>sbrk = (i, si)\<close>
+        \<open>s = (brk, sbrk)\<close> and
+      [simp]: \<open>xs ! i \<notin># dom_m N\<close> \<open>xs' ! i' \<notin># dom_m N'\<close>
+    for s s' brk' sbrk' i' si' N' xs' brk sbrk i si N xs
+      TM TN TD TNE TUE TQ TW SM SN SD SNE SUE SQ SW xs0 xs0' S T
+  proof -
+    have st:
+      \<open>si' = (N', xs')\<close>
+      \<open>sbrk' = (i', N', xs')\<close>
+      \<open>s' = (brk', i', N', xs')\<close>
+      \<open>si = (N', xs')\<close>
+      \<open>sbrk = (i', N', xs')\<close>
+      \<open>s = (brk, i', N', xs')\<close>
+      \<open>i = i'\<close>
+      \<open>N = N'\<close>
+      \<open>xs = xs'\<close>
+      \<open>brk =brk'\<close> and
+      \<open>mark_to_delete_clauses_wl_D_inv S xs0 (brk, i', N', xs')\<close>
+      using st ss' by auto
+    have post: \<open>mark_to_delete_clauses_wl_inv (SM, SN, SD, SNE, SUE, SQ, SW) xs0'
+     (brk', i', N', butlast (xs'[i' := last xs']))\<close>
+      using post_inv unfolding st
+      by auto
+    then have \<open>mark_to_delete_clauses_wl_D_inv S xs0 (brk', i', N', butlast (xs'[i' := last xs']))\<close>
+      using inv xs unfolding mark_to_delete_clauses_wl_D_inv_def prod.case S st
+      by auto
+    then show ?thesis
+      by (auto simp: st)
+  qed
+  have Lit_inL: \<open>N \<propto> (xs ! i) ! 0 \<in># \<L>\<^sub>a\<^sub>l\<^sub>l\<close>
+    if
+      T: \<open>T = (SM, SN, SD, SNE, SUE, SQ, SW)\<close> and
+      S: \<open>S = (SM, SN, SD, SNE, SUE, SQ, SW)\<close> and
+      ss': \<open>(s, s') \<in> {((brk, i, N, xs), brk', i', N', xs'). brk = brk' \<and> i = i' \<and>
+         N = N' \<and> xs = xs' \<and> mark_to_delete_clauses_wl_D_inv S xs0 (brk, i, N, xs)}\<close> and
+      st:
+        \<open>si' = (N', xs')\<close>
+        \<open>sbrk' = (i', si')\<close>
+        \<open>s' = (brk', sbrk')\<close>
+        \<open>si = (N, xs)\<close>
+        \<open>sbrk = (i, si)\<close>
+        \<open>s = (brk, sbrk)\<close> and
+      dom: \<open>\<not> xs ! i \<notin># dom_m N\<close> and
+      \<open>\<not> xs' ! i' \<notin># dom_m N'\<close> and
+    le: \<open>0 < length (N \<propto> (xs ! i))\<close>
+    for s s' brk' sbrk' i' si' N' xs' brk sbrk i si N xs
+      TM TN TD TNE TUE TQ TW SM SN SD SNE SUE SQ SW xs0 xs0' S T
+  proof -
+    have st:
+      \<open>si' = (N', xs')\<close>
+      \<open>sbrk' = (i', N', xs')\<close>
+      \<open>s' = (brk', i', N', xs')\<close>
+      \<open>si = (N', xs')\<close>
+      \<open>sbrk = (i', N', xs')\<close>
+      \<open>s = (brk, i', N', xs')\<close>
+      \<open>i = i'\<close>
+      \<open>N = N'\<close>
+      \<open>xs = xs'\<close>
+      \<open>brk =brk'\<close> and
+      inv_x: \<open>mark_to_delete_clauses_wl_D_inv S xs0 (brk, i', N', xs')\<close>
+      using st ss' by auto
+    have \<open>literals_are_\<L>\<^sub>i\<^sub>n  (SM, N', SD, SNE, SUE, SQ, SW)\<close>
+      using inv_x unfolding mark_to_delete_clauses_wl_D_inv_def prod.case S
+      by fast
+    then have \<open>literals_are_in_\<L>\<^sub>i\<^sub>n (mset (N \<propto> (xs ! i)))\<close>
+      using literals_are_in_\<L>\<^sub>i\<^sub>n_nth[of \<open>xs!i\<close> \<open>(SM, N', SD, SNE, SUE, SQ, SW)\<close>] dom
+      by (auto simp: st)
+    then show ?thesis
+      by (rule literals_are_in_\<L>\<^sub>i\<^sub>n_in_\<L>\<^sub>a\<^sub>l\<^sub>l) (use le in auto)
+  qed
+  have H: \<open>SPEC (\<lambda>N. distinct N)
+       \<le> \<Down> {(N, N'). N=N' \<and> distinct N}
+           (SPEC (\<lambda>N. distinct N))\<close>
+    by (auto intro!: RES_refine)
+  have removed: \<open>((break1, i + 1, fmdrop (xs ! i) N, xs), break1', i' + 1,
+       fmdrop (xs' ! i') N', xs')
+      \<in> {((brk, i, N, xs), brk', i', N', xs').
+          brk = brk' \<and>
+          i = i' \<and>
+          N = N' \<and>
+          xs = xs' \<and> mark_to_delete_clauses_wl_D_inv S xs0 (brk, i, N, xs)}\<close>
+    if
+      \<open>T = (SM, SN, SD, SNE, SUE, SQ, SW)\<close> and
+      S: \<open>S = (SM, SN, SD, SNE, SUE, SQ, SW)\<close> and
+      \<open>literals_are_\<L>\<^sub>i\<^sub>n (SM, SN, SD, SNE, SUE, SQ, SW)\<close> and
+      pre: \<open>mark_to_delete_clauses_wl_D_pre (SM, SN, SD, SNE, SUE, SQ, SW)\<close> and
+      xs0_xs0': \<open>(xs0, xs0') \<in> {(N, N'). N = N' \<and> distinct N}\<close> and
+      \<open>xs0 \<in> {N. distinct N}\<close> and
+      \<open>xs0' \<in> {N. distinct N}\<close> and
+      ss': \<open>(s, s') \<in> {((brk, i, N, xs), brk', i', N', xs'). brk = brk' \<and> i = i' \<and> N = N' \<and>
+         xs = xs' \<and> mark_to_delete_clauses_wl_D_inv S xs0 (brk, i, N, xs)}\<close> and
+      \<open>case s of (brk, i, N, xs) \<Rightarrow> \<not> brk \<and> i < length xs\<close> and
+      \<open>case s' of (brk, i, N, xs) \<Rightarrow> \<not> brk \<and> i < length xs\<close> and
+      inv: \<open>mark_to_delete_clauses_wl_D_inv (SM, SN, SD, SNE, SUE, SQ, SW) xs0 s\<close> and
+      \<open>mark_to_delete_clauses_wl_inv (SM, SN, SD, SNE, SUE, SQ, SW) xs0' s'\<close> and
+      post: \<open>(case s' of
+      (brk, i, N, xs) \<Rightarrow>
+        if xs ! i \<notin># dom_m N
+        then RETURN (brk, i, N, delete_index_and_swap xs i)
+        else ASSERT (0 < length (N \<propto> (xs ! i))) \<bind>
+             (\<lambda>_. SPEC
+                   (\<lambda>b. b \<longrightarrow>
+                        Propagated (N \<propto> (xs ! i) ! 0) (xs ! i) \<notin> set SM \<and>
+                        \<not> irred N (xs ! i)) \<bind>
+                  (\<lambda>can_del.
+                      SPEC (\<lambda>_. True) \<bind>
+                      (\<lambda>brk. ASSERT (i < length xs) \<bind>
+                             (\<lambda>_. if can_del
+                                  then RETURN
+ (brk, i + 1, fmdrop (xs ! i) N, xs)
+                                  else RETURN (brk, i + 1, N, xs))))))
+     \<le> SPEC (mark_to_delete_clauses_wl_inv (SM, SN, SD, SNE, SUE, SQ, SW)
+               xs0')\<close> and
+      s:
+        \<open>si' = (N', xs')\<close>
+        \<open>sbrk' = (i', si')\<close>
+        \<open>s' = (brk', sbrk')\<close>
+        \<open>si = (N, xs)\<close>
+        \<open>sbrk = (i, si)\<close>
+        \<open>s = (brk, sbrk)\<close> and
+      dom: \<open>\<not> xs ! i \<notin># dom_m N\<close> and
+      \<open>\<not> xs' ! i' \<notin># dom_m N'\<close> and
+      length: \<open>0 < length (N' \<propto> (xs' ! i'))\<close> and
+      \<open>0 < length (N \<propto> (xs ! i))\<close> and
+      \<open>N \<propto> (xs ! i) ! 0 \<in># \<L>\<^sub>a\<^sub>l\<^sub>l\<close> and
+      can_del: \<open>can_del \<in> {b. b \<longrightarrow>
+            Propagated (N \<propto> (xs ! i) ! 0) (xs ! i) \<notin> set SM \<and>
+            \<not> irred N (xs ! i)}\<close> and
+      can_del': \<open>can_del' \<in> {b. b \<longrightarrow>
+            Propagated (N' \<propto> (xs' ! i') ! 0) (xs' ! i') \<notin> set SM \<and>
+            \<not> irred N' (xs' ! i')}\<close> and
+      s':
+        \<open>(break1, break1') \<in> bool_rel\<close>
+        \<open>(can_del, can_del') \<in> bool_rel\<close> and
+      \<open>break1 \<in> {_. True}\<close> and
+      \<open>break1' \<in> {_. True}\<close> and
+      i'_le: \<open>i' < length xs'\<close> and
+      \<open>i < length xs\<close> and
+      [simp]: \<open>can_del\<close> and
+      \<open>can_del'\<close>
+    for s s' brk' sbrk' i' si' N' xs' brk sbrk i si N xs can_del can_del' break1 break1'
+      TM TN TD TNE TUE TQ TW SM SN SD SNE SUE SQ SW xs0 xs0' S T
+  proof -
+    have st:
+      \<open>si' = (N', xs')\<close>
+      \<open>sbrk' = (i', N', xs')\<close>
+      \<open>s' = (brk', i', N', xs')\<close>
+      \<open>si = (N, xs)\<close>
+      \<open>sbrk = (i, N, xs)\<close>
+      \<open>s = (brk, i, N, xs)\<close>
+      \<open>xs0 = xs0'\<close>
+      \<open>break1 = break1'\<close>
+      \<open>can_del = can_del'\<close>
+      \<open>i = i'\<close>
+      \<open>N = N'\<close>
+      \<open>xs = xs'\<close> and
+      [simp]: \<open>can_del'\<close>
+      using s s' xs0_xs0' ss'
+      by auto
+    have 1: \<open>(if can_del then RETURN (brk, i' + 1, fmdrop (xs' ! i') N', xs')
+               else RETURN (brk, i' + 1, N', xs')) =
+       RETURN (if can_del then (brk, i' + 1, fmdrop (xs' ! i') N', xs')
+               else (brk, i' + 1, N', xs'))\<close> for can_del brk
+      by auto
+    have \<open>\<not>irred N' (xs' ! i') \<Longrightarrow> \<not>Propagated (N' \<propto> (xs' ! i') ! 0) (xs' ! i') \<in> set SM \<Longrightarrow>
+        \<forall>x\<in>range (\<lambda>brk. (brk, Suc i', fmdrop (xs' ! i') N', xs')) \<union>
+        range (\<lambda>brk. (brk, Suc i', N', xs')).
+       mark_to_delete_clauses_wl_inv (SM, SN, SD, SNE, SUE, SQ, SW) xs0' x\<close> and
+      \<open>mark_to_delete_clauses_wl_inv (SM, SN, SD, SNE, SUE, SQ, SW) xs0'
+            (break1, Suc i', N', xs')\<close>
+      using post dom length i'_le can_del
+      by (auto simp: st 1 RES_RETURN_RES RES_RES_RETURN_RES Union_bool_expand subset_Collect_conv
+          split: if_splits)
+    then have st': \<open>mark_to_delete_clauses_wl_inv (SM, SN, SD, SNE, SUE, SQ, SW) xs0'
+       (break1', Suc i', fmdrop (xs' ! i') N', xs')\<close>
+      using dom length i'_le can_del'
+      by (auto simp: st 1 RES_RETURN_RES RES_RES_RETURN_RES Union_bool_expand subset_Collect_conv
+          split: if_splits)
+    then obtain a aa ab ac ad ae b af ba c d e f g U' where
+      SU: \<open>((SM, SN, SD, SNE, SUE, SQ, SW), af, ba, c, d, e, f, g) \<in> state_wl_l None\<close> and
+        \<open>partial_correct_watching (SM, SN, SD, SNE, SUE, SQ, SW)\<close> and
+      rem: \<open>remove_one_annot_true_clause\<^sup>*\<^sup>* (af, ba, c, d, e, f, g)
+          (af, fmdrop (xs' ! i') N', c, d, e, f, g)\<close> and
+       \<open>filter_mset (\<lambda>i. i \<in># dom_m (fmdrop (xs' ! i') N')) (mset xs') =
+             filter_mset (\<lambda>i. i \<in># dom_m (fmdrop (xs' ! i') N')) (mset xs0')\<close> and
+        \<open>distinct xs'\<close> and
+      list_invs_U: \<open>twl_list_invs (af, ba, c, d, e, f, g)\<close> and
+      confl: \<open>get_conflict_l (af, ba, c, d, e, f, g) = None\<close> and
+      upd: \<open>clauses_to_update_l (af, ba, c, d, e, f, g) = {#}\<close> and
+      UU': \<open>((af, ba, c, d, e, f, g), U') \<in> twl_st_l None\<close> and
+      struct_U': \<open>twl_struct_invs U'\<close>
+      unfolding mark_to_delete_clauses_wl_inv_def prod.case mark_to_delete_clauses_l_inv_def
+      apply -
+      apply normalize_goal+
+      apply (case_tac x)
+      apply clarify
+      by blast
+    obtain V where
+     \<open>cdcl_twl_restart_l\<^sup>*\<^sup>* (af, ba, c, d, e, f, g)
+        (af, fmdrop (xs' ! i') N', c, d, e, f, g)\<close> and
+     UV: \<open>((af, fmdrop (xs' ! i') N', c, d, e, f, g), V)
+       \<in> twl_st_l None\<close> and
+     U'V: \<open>cdcl_twl_restart\<^sup>*\<^sup>* U' V\<close> and
+     \<open>twl_struct_invs V\<close>
+      using rtranclp_remove_one_annot_true_clause_cdcl_twl_restart_l2[OF rem list_invs_U confl upd
+          UU' struct_U']
+      by blast
+    have lits: \<open>literals_are_\<L>\<^sub>i\<^sub>n (SM, SN, SD, SNE, SUE, SQ, SW)\<close>
+      using inv pre unfolding mark_to_delete_clauses_wl_D_pre_def prod.case s by fast+
+    have SV: \<open>((SM, fmdrop (xs' ! i') N', SD, SNE, SUE, SQ, SW), af, fmdrop (xs' ! i') N', c, d, e, f, g) \<in> state_wl_l None\<close>
+      using SU by (auto simp: state_wl_l_def)
+    have \<open>literals_are_\<L>\<^sub>i\<^sub>n (SM, fmdrop (xs' ! i') N', SD, SNE, SUE, SQ, SW)\<close>
+      using cdcl_twl_restart_is_\<L>\<^sub>a\<^sub>l\<^sub>l[OF U'V struct_U' ] lits SU UU' UV SV
+      by (auto simp del: get_clauses.simps get_clauses_wl.simps get_clauses_l.simps
+          unit_clss.simps get_unit_clauses_l.simps get_unit_clauses_wl.simps
+          simp: mset_take_mset_drop_mset')
+    then have \<open>mark_to_delete_clauses_wl_D_inv S xs0' (break1', Suc i', fmdrop (xs' ! i') N', xs')\<close>
+      using st' unfolding mark_to_delete_clauses_wl_D_inv_def S prod.case
+      by auto
+    then show ?thesis
+      by (auto simp: st)
+  qed
+  have kept: \<open>((break1, i + 1, N, xs), break1', i' + 1, N', xs')
+      \<in> {((brk, i, N, xs), brk', i', N', xs').
+          brk = brk' \<and>
+          i = i' \<and>
+          N = N' \<and>
+          xs = xs' \<and>
+          mark_to_delete_clauses_wl_D_inv S xs0
+           (brk, i, N, xs)}\<close>
+    if
+      T: \<open>T = (SM, SN, SD, SNE, SUE, SQ, SW)\<close> and
+      S: \<open>S = (SM, SN, SD, SNE, SUE, SQ, SW)\<close> and
+      \<open>literals_are_\<L>\<^sub>i\<^sub>n (SM, SN, SD, SNE, SUE, SQ, SW)\<close> and
+      \<open>mark_to_delete_clauses_wl_pre (SM, SN, SD, SNE, SUE, SQ, SW)\<close> and
+      pre: \<open>mark_to_delete_clauses_wl_D_pre (SM, SN, SD, SNE, SUE, SQ, SW)\<close> and
+      xs0_xs0': \<open>(xs0, xs0') \<in> {(N, N'). N = N' \<and> distinct N}\<close> and
+      \<open>xs0 \<in> {N. distinct N}\<close> and
+      \<open>xs0' \<in> {N. distinct N}\<close> and
+      ss': \<open>(s, s') \<in> {((brk, i, N, xs), brk', i', N', xs'). brk = brk' \<and> i = i' \<and>
+         N = N' \<and> xs = xs' \<and> mark_to_delete_clauses_wl_D_inv S xs0 (brk, i, N, xs)}\<close> and
+      \<open>case s of (brk, i, N, xs) \<Rightarrow> \<not> brk \<and> i < length xs\<close> and
+      \<open>case s' of (brk, i, N, xs) \<Rightarrow> \<not> brk \<and> i < length xs\<close> and
+      \<open>mark_to_delete_clauses_wl_D_inv (SM, SN, SD, SNE, SUE, SQ, SW) xs0 s\<close> and
+      \<open>mark_to_delete_clauses_wl_inv (SM, SN, SD, SNE, SUE, SQ, SW) xs0' s'\<close> and
+      post: \<open>(case s' of (brk, i, N, xs) \<Rightarrow> if xs ! i \<notin># dom_m N
+        then RETURN (brk, i, N, delete_index_and_swap xs i)
+        else ASSERT (0 < length (N \<propto> (xs ! i))) \<bind>
+             (\<lambda>_. SPEC
+                   (\<lambda>b. b \<longrightarrow>
+                        Propagated (N \<propto> (xs ! i) ! 0)
+                         (xs ! i)
+                        \<notin> set SM \<and>
+                        \<not> irred N (xs ! i)) \<bind>
+                  (\<lambda>can_del.
+                      SPEC (\<lambda>_. True) \<bind>
+                      (\<lambda>brk. ASSERT (i < length xs) \<bind>
+                             (\<lambda>_.
+  if can_del then RETURN (brk, i + 1, fmdrop (xs ! i) N, xs)
+  else RETURN (brk, i + 1, N, xs))))))
+     \<le> SPEC
+         (mark_to_delete_clauses_wl_inv
+           (SM, SN, SD, SNE, SUE, SQ, SW) xs0')\<close> and
+      s:
+        \<open>si' = (N', xs')\<close>
+        \<open>sbrk' = (i', si')\<close>
+        \<open>s' = (brk', sbrk')\<close>
+        \<open>si = (N, xs)\<close>
+        \<open>sbrk = (i, si)\<close>
+        \<open>s = (brk, sbrk)\<close> and
+      dom: \<open>\<not> xs ! i \<notin># dom_m N\<close> and
+      \<open>\<not> xs' ! i' \<notin># dom_m N'\<close> and
+      length: \<open>0 < length (N' \<propto> (xs' ! i'))\<close> and
+      \<open>0 < length (N \<propto> (xs ! i))\<close> and
+      \<open>N \<propto> (xs ! i) ! 0 \<in># \<L>\<^sub>a\<^sub>l\<^sub>l\<close> and
+      \<open>can_del
+     \<in> {b. b \<longrightarrow>
+            Propagated (N \<propto> (xs ! i) ! 0) (xs ! i) \<notin> set SM \<and>
+            \<not> irred N (xs ! i)}\<close> and
+      \<open>can_del' \<in> {b. b \<longrightarrow>
+            Propagated (N' \<propto> (xs' ! i') ! 0) (xs' ! i')
+            \<notin> set SM \<and>
+            \<not> irred N' (xs' ! i')}\<close> and
+      s':
+        \<open>(break1, break1') \<in> bool_rel\<close>
+        \<open>(can_del, can_del') \<in> bool_rel\<close> and
+      \<open>break1 \<in> {_. True}\<close> and
+      \<open>break1' \<in> {_. True}\<close> and
+      i'_le: \<open>i' < length xs'\<close> and
+      \<open>i < length xs\<close> and
+      can_del: \<open>\<not> can_del\<close> and
+      \<open>\<not> can_del'\<close>
+    for s s' brk' sbrk' i' si' N' xs' brk sbrk i si N xs can_del can_del' break1 break1'
+      TM TN TD TNE TUE TQ TW SM SN SD SNE SUE SQ SW xs0 xs0' S T
+  proof -
+    have st:
+      \<open>si' = (N', xs')\<close>
+      \<open>sbrk' = (i', N', xs')\<close>
+      \<open>s' = (brk', i', N', xs')\<close>
+      \<open>si = (N, xs)\<close>
+      \<open>sbrk = (i, N, xs)\<close>
+      \<open>s = (brk, i, N, xs)\<close>
+      \<open>xs0 = xs0'\<close>
+      \<open>break1 = break1'\<close>
+      \<open>can_del = can_del'\<close>
+      \<open>i = i'\<close>
+      \<open>N = N'\<close>
+      \<open>xs = xs'\<close> and
+      [simp]: \<open>can_del' = False\<close>
+      using s s' xs0_xs0' ss' can_del
+      by auto
+    have 1: \<open>(if can_del then RETURN (brk, i' + 1, fmdrop (xs' ! i') N', xs')
+               else RETURN (brk, i' + 1, N', xs')) =
+       RETURN (if can_del then (brk, i' + 1, fmdrop (xs' ! i') N', xs')
+               else (brk, i' + 1, N', xs'))\<close> for can_del brk
+      by auto
+    have \<open>\<not>irred N' (xs' ! i') \<Longrightarrow> \<not>Propagated (N' \<propto> (xs' ! i') ! 0) (xs' ! i') \<in> set SM \<Longrightarrow>
+        \<forall>x\<in>range (\<lambda>brk. (brk, Suc i', fmdrop (xs' ! i') N', xs')) \<union>
+        range (\<lambda>brk. (brk, Suc i', N', xs')).
+       mark_to_delete_clauses_wl_inv (SM, SN, SD, SNE, SUE, SQ, SW) xs0' x\<close> and
+      \<open>mark_to_delete_clauses_wl_inv (SM, SN, SD, SNE, SUE, SQ, SW) xs0'
+            (break1, Suc i', N', xs')\<close>
+      using post dom length i'_le can_del
+      by (auto simp: st 1 RES_RETURN_RES RES_RES_RETURN_RES Union_bool_expand subset_Collect_conv
+          split: if_splits)
+    then have st': \<open>mark_to_delete_clauses_wl_inv (SM, SN, SD, SNE, SUE, SQ, SW) xs0'
+       (break1', Suc i', N', xs')\<close>
+      using dom length i'_le
+      by (auto simp: st 1 RES_RETURN_RES RES_RES_RETURN_RES Union_bool_expand subset_Collect_conv
+          split: if_splits)
+    then obtain a aa ab ac ad ae b af ba c d e f g U' where
+    \<open>distinct xs'\<close> and
+      SU: \<open>((SM, SN, SD, SNE, SUE, SQ, SW), af, ba, c, d, e, f, g) \<in> state_wl_l None\<close> and
+      \<open>partial_correct_watching (SM, SN, SD, SNE, SUE, SQ, SW)\<close> and
+      rem: \<open>remove_one_annot_true_clause\<^sup>*\<^sup>* (af, ba, c, d, e, f, g)
+          (af, N', c, d, e, f, g)\<close> and
+      \<open>filter_mset (\<lambda>i. i \<in># dom_m N') (mset xs') =
+             filter_mset (\<lambda>i. i \<in># dom_m N') (mset xs0')\<close> and
+      \<open>distinct xs'\<close> and
+      list_invs_U: \<open>twl_list_invs (af, ba, c, d, e, f, g)\<close> and
+      confl: \<open>get_conflict_l (af, ba, c, d, e, f, g) = None\<close> and
+      upd: \<open>clauses_to_update_l (af, ba, c, d, e, f, g) = {#}\<close> and
+      UU': \<open>((af, ba, c, d, e, f, g), U') \<in> twl_st_l None\<close> and
+      struct_U': \<open>twl_struct_invs U'\<close>
+      unfolding mark_to_delete_clauses_wl_inv_def prod.case mark_to_delete_clauses_l_inv_def
+      apply -
+      apply normalize_goal+
+      apply (case_tac x)
+      apply clarify
+      by blast
+    obtain V where
+      \<open>cdcl_twl_restart_l\<^sup>*\<^sup>* (af, ba, c, d, e, f, g) (af, N', c, d, e, f, g)\<close> and
+      UV: \<open>((af, N', c, d, e, f, g), V) \<in> twl_st_l None\<close> and
+      U'V: \<open>cdcl_twl_restart\<^sup>*\<^sup>* U' V\<close> and
+      \<open>twl_struct_invs V\<close>
+      using rtranclp_remove_one_annot_true_clause_cdcl_twl_restart_l2[OF rem list_invs_U confl upd
+          UU' struct_U']
+      by blast
+    have lits: \<open>literals_are_\<L>\<^sub>i\<^sub>n (SM, SN, SD, SNE, SUE, SQ, SW)\<close>
+      using pre unfolding mark_to_delete_clauses_wl_D_pre_def prod.case s by fast+
+    have SV: \<open>((SM, N', SD, SNE, SUE, SQ, SW), af, N', c, d, e, f, g) \<in> state_wl_l None\<close>
+      using SU by (auto simp: state_wl_l_def)
+    have \<open>literals_are_\<L>\<^sub>i\<^sub>n (SM, N', SD, SNE, SUE, SQ, SW)\<close>
+      using cdcl_twl_restart_is_\<L>\<^sub>a\<^sub>l\<^sub>l[OF U'V struct_U' ] lits SU UU' UV SV
+      by (auto simp del: get_clauses.simps get_clauses_wl.simps get_clauses_l.simps
+          unit_clss.simps get_unit_clauses_l.simps get_unit_clauses_wl.simps
+          simp: mset_take_mset_drop_mset')
+    then have \<open>mark_to_delete_clauses_wl_D_inv S xs0' (break1', Suc i', N', xs')\<close>
+      using st' unfolding mark_to_delete_clauses_wl_D_inv_def S prod.case
+      by auto
+    then show ?thesis
+      by (auto simp: st)
+  qed
+  have refine_ASSERT:
+    \<open>(\<Phi> \<Longrightarrow> \<Psi>) \<Longrightarrow> (\<Phi> \<Longrightarrow> \<Psi> \<Longrightarrow> P \<le> \<Down> R Q) \<Longrightarrow>
+         do {ASSERT \<Psi>; P} \<le> \<Down> R (do {ASSERT \<Phi>; Q})\<close> for P Q \<Phi> \<Psi> R
+    by refine_vcg auto
   show ?thesis
     unfolding uncurry_def mark_to_delete_clauses_wl_D_def mark_to_delete_clauses_wl_def
+      collect_valid_indices_wl_def
     apply (intro frefI nres_relI)
     subgoal for S T
-      apply (refine_vcg
-          remove_one_annot_true_clause_imp_wl_D_remove_one_annot_true_clause_imp_wl[THEN fref_to_Down]
-          remove_one_annot_true_clause_one_imp_wl_D_remove_one_annot_true_clause_one_imp_wl[THEN fref_to_Down_curry]
-          WHILEIT_refine_with_post[where R = \<open>{((brk, i, N), (brk', i', N')). brk = brk' \<and> i=i' \<and> N=N' \<and>
-            mark_to_delete_clauses_wl_D_inv S (brk, i, N)}\<close>])
+      apply (cases S; cases T)
+      apply (clarify)
+      apply (rule refine_ASSERT)
       subgoal unfolding mark_to_delete_clauses_wl_D_pre_def by auto
-      subgoal for S S' T T'
-        by (auto simp: remove_one_annot_true_clause_imp_wl_D_inv_def)
-      subgoal unfolding mark_to_delete_clauses_wl_D_inv_def by auto
-      subgoal by auto
-      subgoal by auto
-      subgoal by auto
-      subgoal by auto
-      subgoal by auto
-      subgoal by auto
-      subgoal by auto
-      subgoal apply (auto simp: intro_spec_iff mark_to_delete_clauses_wl_D_inv_def
-            split: ) sorry
-      subgoal by (auto simp: intro_spec_iff mark_to_delete_clauses_wl_D_inv_def)
-      subgoal unfolding mark_to_delete_clauses_wl_D_inv_def by auto
+      apply (rule bind_refine_RES(3)[OF H])
+      subgoal for TM TN TD TNE TUE TQ TW SM SN SD SNE SUE SQ SW xs0 xs0'
+        apply (refine_vcg
+            remove_one_annot_true_clause_imp_wl_D_remove_one_annot_true_clause_imp_wl[THEN fref_to_Down]
+            remove_one_annot_true_clause_one_imp_wl_D_remove_one_annot_true_clause_one_imp_wl[THEN fref_to_Down_curry]
+            WHILEIT_refine_with_post[where R = \<open>{((brk, i, N, xs), (brk', i', N', xs')). brk = brk' \<and>
+              i=i' \<and> N=N' \<and> xs = xs' \<and>
+              mark_to_delete_clauses_wl_D_inv S xs0 (brk, i, N, xs)}\<close>])
+        subgoal unfolding mark_to_delete_clauses_wl_D_inv_def by auto
+        subgoal unfolding mark_to_delete_clauses_wl_D_inv_def by auto
+        subgoal by auto
+        subgoal by auto
+        subgoal by (rule R_notin)
+        subgoal by auto
+        subgoal by (rule Lit_inL)
+        subgoal by auto
+        subgoal by auto
+        subgoal by auto
+        subgoal by auto
+        subgoal by (rule removed)
+        subgoal by (rule kept)
+        subgoal unfolding mark_to_delete_clauses_wl_D_inv_def by auto
+        done
       done
     done
 qed
 
-definition cdcl_twl_restart_wl_prog_D :: \<open>nat twl_st_wl \<Rightarrow> nat twl_st_wl nres\<close> where
-\<open>cdcl_twl_restart_wl_prog_D S = do {
-    S \<leftarrow> remove_one_annot_true_clause_imp_wl_D S;
-    mark_to_delete_clauses_wl_D S
-  }\<close>
-
-lemma cdcl_twl_restart_wl_prog_D_cdcl_twl_restart_wl_prog:
-  \<open>(cdcl_twl_restart_wl_prog_D, cdcl_twl_restart_wl_prog) \<in>
-   {(S, T). (S, T) \<in> Id \<and> literals_are_\<L>\<^sub>i\<^sub>n S} \<rightarrow>\<^sub>f
-     \<langle>{(S, T). (S, T) \<in> Id \<and> literals_are_\<L>\<^sub>i\<^sub>n S}\<rangle>nres_rel\<close>
-proof -
-  show ?thesis
-    unfolding uncurry_def cdcl_twl_restart_wl_prog_D_def cdcl_twl_restart_wl_prog_def
-    apply (intro frefI nres_relI)
-    by (refine_vcg
-      remove_one_annot_true_clause_imp_wl_D_remove_one_annot_true_clause_imp_wl[THEN fref_to_Down]
-      remove_one_annot_true_clause_one_imp_wl_D_remove_one_annot_true_clause_one_imp_wl[THEN fref_to_Down_curry]
-      mark_to_delete_clauses_wl_D_mark_to_delete_clauses_wl[THEN fref_to_Down])
-qed
 
 definition rewatch_clause_D
   :: \<open>nat clauses_l \<Rightarrow> nat \<Rightarrow> (nat literal \<Rightarrow> watched) \<Rightarrow> (nat literal \<Rightarrow> watched) nres\<close>
@@ -529,13 +948,6 @@ where
     ASSERT(L' \<in># \<L>\<^sub>a\<^sub>l\<^sub>l);
     RETURN (W(L := W L @ [C], L' := W L' @ [C]))
   }\<close>
-
-(* TODO Move *)
-lemma literals_are_in_\<L>\<^sub>i\<^sub>n_in_\<L>\<^sub>a\<^sub>l\<^sub>l:
-  \<open>literals_are_in_\<L>\<^sub>i\<^sub>n C \<Longrightarrow> L \<in># C \<Longrightarrow> L \<in># \<L>\<^sub>a\<^sub>l\<^sub>l\<close>
-  unfolding literals_are_in_\<L>\<^sub>i\<^sub>n_def
-  by (auto dest!: multi_member_split simp: all_lits_of_m_add_mset)
-(* End Move *)
 
 lemma rewatch_clause_D_rewatch_clause:
   \<open>(uncurry2 rewatch_clause_D, uncurry2 rewatch_clause) \<in>
@@ -580,7 +992,7 @@ proof -
   show ?thesis
     unfolding rewatch_clauses_prog_D_def rewatch_clauses_prog_def
     apply (intro frefI nres_relI)
-    apply (refine_rcg 
+    apply (refine_rcg
      rewatch_clause_D_rewatch_clause[THEN fref_to_Down_curry2]
       WHILEIT_refine[where R = \<open>nat_rel \<times>\<^sub>f (Id :: ((nat literal \<Rightarrow> watched) \<times> _) set) \<close>])
     subgoal unfolding rewatch_clauses_prog_D_pre_def by auto
@@ -590,7 +1002,7 @@ proof -
     subgoal by auto
     subgoal by auto
     subgoal by auto
-    subgoal unfolding rewatch_clauses_prog_D_pre_def 
+    subgoal unfolding rewatch_clauses_prog_D_pre_def
       by (auto dest!: literals_are_in_\<L>\<^sub>i\<^sub>n_nth[of _ \<open>(M, N, D, NE, UE, Q, W0)\<close> for M N D NE UE Q W0,
             simplified])
     subgoal by auto
@@ -599,6 +1011,79 @@ proof -
     subgoal by auto
     done
 qed
+
+
+definition mark_to_delete_clauses_wl_D_post where
+  \<open>mark_to_delete_clauses_wl_D_post S T \<longleftrightarrow>
+     (mark_to_delete_clauses_wl_post S T \<and> literals_are_\<L>\<^sub>i\<^sub>n S)\<close>
+
+definition cdcl_twl_restart_wl_prog_D :: \<open>nat twl_st_wl \<Rightarrow> nat twl_st_wl nres\<close> where
+\<open>cdcl_twl_restart_wl_prog_D S = do {
+    S \<leftarrow> remove_one_annot_true_clause_imp_wl_D S;
+    ASSERT(mark_to_delete_clauses_wl_D_pre S);
+    T \<leftarrow> mark_to_delete_clauses_wl_D S;
+    rewatch_clauses_prog_D T
+  }\<close>
+
+lemma cdcl_twl_restart_wl_prog_D_cdcl_twl_restart_wl_prog:
+  \<open>(cdcl_twl_restart_wl_prog_D, cdcl_twl_restart_wl_prog) \<in>
+   {(S, T). (S, T) \<in> Id \<and> literals_are_\<L>\<^sub>i\<^sub>n S} \<rightarrow>\<^sub>f
+     \<langle>{(S, T). (S, T) \<in> Id \<and> literals_are_\<L>\<^sub>i\<^sub>n S}\<rangle>nres_rel\<close>
+proof -
+  have [refine0]: \<open>rewatch_clauses_prog_D U
+      \<le> \<Down> {(S, T). (S, T) \<in> Id \<and> literals_are_\<L>\<^sub>i\<^sub>n S}
+          (rewatch_clauses U')\<close>
+    if
+      UU': \<open>(U, U') \<in> {(S, T). (S, T) \<in> Id \<and> literals_are_\<L>\<^sub>i\<^sub>n S}\<close> and
+      post: \<open>mark_to_delete_clauses_wl_post T' U'\<close>
+    for S S' T T' U U'
+  proof -
+    have le: \<open>rewatch_clauses_prog_D U \<le> \<Down> {(S, T). (S, T) \<in> Id \<and> literals_are_\<L>\<^sub>i\<^sub>n S}
+            (rewatch_clauses_prog U')\<close>
+      using rewatch_clauses_prog_D_rewatch_clauses_prog[THEN fref_to_Down, of U U']
+        UU' by auto
+    obtain x xa xb where
+      \<open>(T', x) \<in> state_wl_l None\<close> and
+      U'_xa: \<open>(U', xa) \<in> state_wl_l None\<close> and
+      xxb: \<open>(x, xb) \<in> twl_st_l None\<close> and
+      rem: \<open>remove_one_annot_true_clause\<^sup>*\<^sup>* x xa\<close> and
+      list_invs: \<open>twl_list_invs x\<close> and
+      struct_xb: \<open>twl_struct_invs xb\<close> and
+      part_T': \<open>partial_correct_watching T'\<close> and
+      confl: \<open>get_conflict_l x = None\<close> and
+      upd: \<open>clauses_to_update_l x = {#}\<close> and
+      \<open>partial_correct_watching T'\<close> and
+      part_U': \<open>partial_correct_watching U'\<close>
+      using post unfolding mark_to_delete_clauses_wl_post_def mark_to_delete_clauses_l_post_def
+      by blast
+    obtain xc where
+      xa_xc: \<open>(xa, xc) \<in> twl_st_l None\<close> and
+      struct_xc: \<open>twl_struct_invs xc\<close> and
+      x_xa: \<open>cdcl_twl_restart_l\<^sup>*\<^sup>* x xa\<close> and
+      \<open>cdcl_twl_restart\<^sup>*\<^sup>* xb xc\<close>
+      using rtranclp_remove_one_annot_true_clause_cdcl_twl_restart_l2[OF rem list_invs confl upd
+          xxb struct_xb]
+      by blast
+    have list_xa: \<open>twl_list_invs xa\<close>
+      using rtranclp_cdcl_twl_restart_l_list_invs[OF x_xa list_invs] .
+    have \<open>rewatch_clauses_prog U' \<le> rewatch_clauses U'\<close>
+      using rewatch_clauses_prog_rewatch_clauses[of U', OF U'_xa xa_xc struct_xc list_xa part_U'] .
+    then show ?thesis
+      using ref_two_step[OF le] by blast
+  qed
+  show ?thesis
+    unfolding uncurry_def cdcl_twl_restart_wl_prog_D_def cdcl_twl_restart_wl_prog_def
+    apply (intro frefI nres_relI)
+    apply (refine_vcg
+      remove_one_annot_true_clause_imp_wl_D_remove_one_annot_true_clause_imp_wl[THEN fref_to_Down]
+      remove_one_annot_true_clause_one_imp_wl_D_remove_one_annot_true_clause_one_imp_wl[THEN fref_to_Down_curry]
+      mark_to_delete_clauses_wl_D_mark_to_delete_clauses_wl[THEN fref_to_Down])
+    subgoal for S T U V
+      unfolding mark_to_delete_clauses_wl_D_pre_def by blast
+    apply assumption
+    done
+qed
+
 
 definition restart_abs_wl_D_pre :: \<open>nat twl_st_wl \<Rightarrow> bool \<Rightarrow> bool\<close> where
   \<open>restart_abs_wl_D_pre S brk \<longleftrightarrow>
@@ -610,9 +1095,7 @@ definition restart_prog_wl_D :: "nat twl_st_wl \<Rightarrow> nat \<Rightarrow> b
      b \<leftarrow> restart_required_wl S n;
      if b \<and> \<not>brk then do {
        T \<leftarrow> cdcl_twl_restart_wl_prog_D S;
-       ASSERT(literals_are_\<L>\<^sub>i\<^sub>n S);
-       U \<leftarrow> rewatch_clauses_prog_D T;
-       RETURN (U, n + 1)
+       RETURN (T, n + 1)
      }
      else
        RETURN (S, n)
@@ -627,17 +1110,6 @@ proof -
     if \<open>(x1c, x1a) \<in> Id\<close> \<open>(x2b, x2) \<in> Id\<close>
     for x1c x1a x2b x2
     using that by auto
-  have \<open>(T, T') \<in> {(S, T). (S, T) \<in> Id \<and> literals_are_\<L>\<^sub>i\<^sub>n S} \<Longrightarrow> 
-      rewatch_clauses_prog_D T \<le> \<Down> {(S, T). (S, T) \<in> Id \<and> literals_are_\<L>\<^sub>i\<^sub>n S} (rewatch_clauses T')\<close>
-    for T T'
-    apply (rule order.trans)
-    apply (rule rewatch_clauses_prog_D_rewatch_clauses_prog[THEN fref_to_Down, of T T']; 
-     assumption?; fast)
-
-    using 
-      rewatch_clauses_prog_D_rewatch_clauses_prog[THEN fref_to_Down, of T T']
-      rewatch_clauses_prog_rewatch_clauses
-
 
   show ?thesis
     unfolding uncurry_def restart_prog_wl_D_def restart_prog_wl_def
@@ -648,8 +1120,6 @@ proof -
       remove_one_annot_true_clause_imp_wl_D_remove_one_annot_true_clause_imp_wl[THEN fref_to_Down]
       cdcl_twl_restart_wl_prog_D_cdcl_twl_restart_wl_prog[THEN fref_to_Down])
     subgoal unfolding restart_abs_wl_D_pre_def by auto
-    subgoal by auto
-    subgoal by auto
     subgoal by auto
     subgoal by auto
     subgoal by auto
@@ -675,6 +1145,27 @@ definition cdcl_twl_stgy_restart_prog_wl_D :: "nat twl_st_wl \<Rightarrow> nat t
     RETURN T
   }\<close>
 
+lemma cdcl_twl_stgy_restart_prog_wl_D_cdcl_twl_stgy_restart_prog_wl:
+  \<open>(cdcl_twl_stgy_restart_prog_wl_D, cdcl_twl_stgy_restart_prog_wl) \<in>
+     {(S, T). (S, T) \<in> Id \<and> literals_are_\<L>\<^sub>i\<^sub>n S} \<rightarrow>\<^sub>f
+     \<langle>{(S, T). (S, T) \<in> Id \<and> literals_are_\<L>\<^sub>i\<^sub>n S}\<rangle>nres_rel\<close>
+  unfolding uncurry_def cdcl_twl_stgy_restart_prog_wl_D_def
+    cdcl_twl_stgy_restart_prog_wl_def
+  apply (intro frefI nres_relI)
+  apply (refine_vcg
+      restart_prog_wl_D_restart_prog_wl[THEN fref_to_Down_curry2]
+      cdcl_twl_o_prog_wl_D_spec'[THEN fref_to_Down]
+      unit_propagation_outer_loop_wl_D_spec'[THEN fref_to_Down]
+      WHILEIT_refine[where R=\<open>bool_rel \<times>\<^sub>r {(S, T). (S, T) \<in> Id \<and> literals_are_\<L>\<^sub>i\<^sub>n S} \<times>\<^sub>r nat_rel\<close>])
+  subgoal by auto
+  subgoal by auto
+  subgoal by auto
+  subgoal by auto
+  subgoal by auto
+  subgoal by auto
+  subgoal by auto
+  subgoal by auto
+  done
 
 end
 
